open import Relation.Binary.PropositionalEquality using (_â‰¡_; refl; cong; congâ‚‚)

data Type : Set where
  ğŸ˜ ğŸ™ âŠ¥ âŠ¤          : Type
  Â¡ Â¿              : Type â†’ Type
  _&_ _âŠ•_ _âŠ—_ _â…‹_  : Type â†’ Type â†’ Type

data Dual : Type â†’ Type â†’ Set where
  d-ğŸ˜-âŠ¤  : Dual ğŸ˜ âŠ¤
  d-âŠ¤-ğŸ˜  : Dual âŠ¤ ğŸ˜
  d-ğŸ™-âŠ¥  : Dual ğŸ™ âŠ¥
  d-âŠ¥-ğŸ™  : Dual âŠ¥ ğŸ™
  d-!-?  : âˆ€{A B} â†’ Dual A B â†’ Dual (Â¡ A) (Â¿ B)
  d-?-!  : âˆ€{A B} â†’ Dual A B â†’ Dual (Â¿ A) (Â¡ B)
  d-&-âŠ•  : âˆ€{A B Aâ€² Bâ€²} â†’ Dual A Aâ€² â†’ Dual B Bâ€² â†’ Dual (A & B) (Aâ€² âŠ• Bâ€²)
  d-âŠ•-&  : âˆ€{A B Aâ€² Bâ€²} â†’ Dual A Aâ€² â†’ Dual B Bâ€² â†’ Dual (A âŠ• B) (Aâ€² & Bâ€²)
  d-âŠ—-â…‹  : âˆ€{A B Aâ€² Bâ€²} â†’ Dual A Aâ€² â†’ Dual B Bâ€² â†’ Dual (A âŠ— B) (Aâ€² â…‹ Bâ€²)
  d-â…‹-âŠ—  : âˆ€{A B Aâ€² Bâ€²} â†’ Dual A Aâ€² â†’ Dual B Bâ€² â†’ Dual (A â…‹ B) (Aâ€² âŠ— Bâ€²)

dual-symm   : âˆ€{A B} â†’ Dual A B â†’ Dual B A
dual-symm d-ğŸ˜-âŠ¤ = d-âŠ¤-ğŸ˜
dual-symm d-âŠ¤-ğŸ˜ = d-ğŸ˜-âŠ¤
dual-symm d-ğŸ™-âŠ¥ = d-âŠ¥-ğŸ™
dual-symm d-âŠ¥-ğŸ™ = d-ğŸ™-âŠ¥
dual-symm (d-!-? p) = d-?-! (dual-symm p)
dual-symm (d-?-! p) = d-!-? (dual-symm p)
dual-symm (d-&-âŠ• p q) = d-âŠ•-& (dual-symm p) (dual-symm q)
dual-symm (d-âŠ•-& p q) = d-&-âŠ• (dual-symm p) (dual-symm q)
dual-symm (d-âŠ—-â…‹ p q) = d-â…‹-âŠ— (dual-symm p) (dual-symm q)
dual-symm (d-â…‹-âŠ— p q) = d-âŠ—-â…‹ (dual-symm p) (dual-symm q)

dual-inv    : âˆ€{A B C} â†’ Dual A B â†’ Dual B C â†’ A â‰¡ C
dual-inv d-ğŸ˜-âŠ¤ d-âŠ¤-ğŸ˜ = refl
dual-inv d-âŠ¤-ğŸ˜ d-ğŸ˜-âŠ¤ = refl
dual-inv d-ğŸ™-âŠ¥ d-âŠ¥-ğŸ™ = refl
dual-inv d-âŠ¥-ğŸ™ d-ğŸ™-âŠ¥ = refl
dual-inv (d-!-? p) (d-?-! q) = cong Â¡ (dual-inv p q)
dual-inv (d-?-! p) (d-!-? q) = cong Â¿ (dual-inv p q)
dual-inv (d-&-âŠ• p q) (d-âŠ•-& r s) = congâ‚‚ _&_ (dual-inv p r) (dual-inv q s)
dual-inv (d-âŠ•-& p q) (d-&-âŠ• r s) = congâ‚‚ _âŠ•_ (dual-inv p r) (dual-inv q s)
dual-inv (d-âŠ—-â…‹ p q) (d-â…‹-âŠ— r s) = congâ‚‚ _âŠ—_ (dual-inv p r) (dual-inv q s)
dual-inv (d-â…‹-âŠ— p q) (d-âŠ—-â…‹ r s) = congâ‚‚ _â…‹_ (dual-inv p r) (dual-inv q s)

dual-fun-r  : âˆ€{A B C} â†’ Dual A B â†’ Dual A C â†’ B â‰¡ C
dual-fun-r d e = dual-inv (dual-symm d) e

dual-fun-l  : âˆ€{A B C} â†’ Dual B A â†’ Dual C A â†’ B â‰¡ C
dual-fun-l d e = dual-inv d (dual-symm e)