open import Relation.Binary.PropositionalEquality using (_â‰¡_; refl; trans; sym; cong; congâ‚‚)
open import Relation.Binary.PropositionalEquality.Properties as Eq
open Eq.â‰¡-Reasoning

open import Data.Nat
open import Data.Fin

data Name (n : â„•) : Set where
  var ort : Fin n -> Name n

data Type : â„• -> Set where
  ğŸ˜ ğŸ™ âŠ¥ âŠ¤          : âˆ€{n} -> Type n
  ref              : âˆ€{n} -> Name n -> Type n
  Â¡ Â¿              : âˆ€{n} -> Type n â†’ Type n
  _&_ _âŠ•_ _âŠ—_ _â…‹_  : âˆ€{n} -> Type n â†’ Type n â†’ Type n
  $âˆ€ $âˆƒ            : âˆ€{n} -> Type (suc n) -> Type n

data Dual : âˆ€{n} -> Type n â†’ Type n â†’ Set where
  d-ğŸ˜-âŠ¤  : âˆ€{n} -> Dual {n} ğŸ˜ âŠ¤
  d-âŠ¤-ğŸ˜  : âˆ€{n} -> Dual {n} âŠ¤ ğŸ˜
  d-ğŸ™-âŠ¥  : âˆ€{n} -> Dual {n} ğŸ™ âŠ¥
  d-âŠ¥-ğŸ™  : âˆ€{n} -> Dual {n} âŠ¥ ğŸ™
  d-!-?  : âˆ€{n} {A B} â†’ Dual {n} A B â†’ Dual (Â¡ A) (Â¿ B)
  d-?-!  : âˆ€{n} {A B} â†’ Dual {n} A B â†’ Dual (Â¿ A) (Â¡ B)
  d-&-âŠ•  : âˆ€{n} {A B Aâ€² Bâ€²} â†’ Dual {n} A Aâ€² â†’ Dual B Bâ€² â†’ Dual (A & B) (Aâ€² âŠ• Bâ€²)
  d-âŠ•-&  : âˆ€{n} {A B Aâ€² Bâ€²} â†’ Dual {n} A Aâ€² â†’ Dual B Bâ€² â†’ Dual (A âŠ• B) (Aâ€² & Bâ€²)
  d-âŠ—-â…‹  : âˆ€{n} {A B Aâ€² Bâ€²} â†’ Dual {n} A Aâ€² â†’ Dual B Bâ€² â†’ Dual (A âŠ— B) (Aâ€² â…‹ Bâ€²)
  d-â…‹-âŠ—  : âˆ€{n} {A B Aâ€² Bâ€²} â†’ Dual {n} A Aâ€² â†’ Dual B Bâ€² â†’ Dual (A â…‹ B) (Aâ€² âŠ— Bâ€²)
  d-âˆ€-âˆƒ  : âˆ€{n} {A B : Type (suc n)} -> Dual A B -> Dual ($âˆ€ A) ($âˆƒ B)
  d-âˆƒ-âˆ€  : âˆ€{n} {A B : Type (suc n)} -> Dual A B -> Dual ($âˆƒ A) ($âˆ€ B)
  d-v-o  : âˆ€{n} {x : Fin n} -> Dual (ref (var x)) (ref (ort x))
  d-o-v  : âˆ€{n} {x : Fin n} -> Dual (ref (ort x)) (ref (var x))

dual-symm : âˆ€{n} {A B : Type n} â†’ Dual A B â†’ Dual B A
dual-symm d-ğŸ˜-âŠ¤ = d-âŠ¤-ğŸ˜
dual-symm d-âŠ¤-ğŸ˜ = d-ğŸ˜-âŠ¤
dual-symm d-ğŸ™-âŠ¥ = d-âŠ¥-ğŸ™
dual-symm d-âŠ¥-ğŸ™ = d-ğŸ™-âŠ¥
dual-symm (d-!-? p) = d-?-! (dual-symm p)
dual-symm (d-?-! p) = d-!-? (dual-symm p)
dual-symm (d-&-âŠ• p q) = d-âŠ•-& (dual-symm p) (dual-symm q)
dual-symm (d-âŠ•-& p q) = d-&-âŠ• (dual-symm p) (dual-symm q)
dual-symm (d-âŠ—-â…‹ p q) = d-â…‹-âŠ— (dual-symm p) (dual-symm q)
dual-symm (d-â…‹-âŠ— p q) = d-âŠ—-â…‹ (dual-symm p) (dual-symm q)
dual-symm (d-âˆ€-âˆƒ p) = d-âˆƒ-âˆ€ (dual-symm p)
dual-symm (d-âˆƒ-âˆ€ p) = d-âˆ€-âˆƒ (dual-symm p)
dual-symm d-v-o = d-o-v
dual-symm d-o-v = d-v-o

dual-inv : âˆ€{n} {A B C : Type n} â†’ Dual A B â†’ Dual B C â†’ A â‰¡ C
dual-inv d-ğŸ˜-âŠ¤ d-âŠ¤-ğŸ˜ = refl
dual-inv d-âŠ¤-ğŸ˜ d-ğŸ˜-âŠ¤ = refl
dual-inv d-ğŸ™-âŠ¥ d-âŠ¥-ğŸ™ = refl
dual-inv d-âŠ¥-ğŸ™ d-ğŸ™-âŠ¥ = refl
dual-inv (d-!-? p) (d-?-! q) = cong Â¡ (dual-inv p q)
dual-inv (d-?-! p) (d-!-? q) = cong Â¿ (dual-inv p q)
dual-inv (d-&-âŠ• p q) (d-âŠ•-& r s) = congâ‚‚ _&_ (dual-inv p r) (dual-inv q s)
dual-inv (d-âŠ•-& p q) (d-&-âŠ• r s) = congâ‚‚ _âŠ•_ (dual-inv p r) (dual-inv q s)
dual-inv (d-âŠ—-â…‹ p q) (d-â…‹-âŠ— r s) = congâ‚‚ _âŠ—_ (dual-inv p r) (dual-inv q s)
dual-inv (d-â…‹-âŠ— p q) (d-âŠ—-â…‹ r s) = congâ‚‚ _â…‹_ (dual-inv p r) (dual-inv q s)
dual-inv (d-âˆ€-âˆƒ p) (d-âˆƒ-âˆ€ q) = cong $âˆ€ (dual-inv p q)
dual-inv (d-âˆƒ-âˆ€ p) (d-âˆ€-âˆƒ q) = cong $âˆƒ (dual-inv p q)
dual-inv d-v-o d-o-v = refl
dual-inv d-o-v d-v-o = refl

dual-fun-r  : âˆ€{n} {A B C : Type n} â†’ Dual A B â†’ Dual A C â†’ B â‰¡ C
dual-fun-r d e = dual-inv (dual-symm d) e

dual-fun-l  : âˆ€{n} {A B C : Type n} â†’ Dual B A â†’ Dual C A â†’ B â‰¡ C
dual-fun-l d e = dual-inv d (dual-symm e)

dualN : âˆ€{n} -> Name n -> Name n
dualN (var x) = ort x
dualN (ort x) = var x

ext : âˆ€{m n} -> (Fin m -> Fin n) -> Fin (suc m) -> Fin (suc n)
ext Ï zero = zero
ext Ï (suc k) = suc (Ï k)

rename : âˆ€{m n} -> (Fin m -> Fin n) -> Type m -> Type n
rename Ï ğŸ˜ = ğŸ˜
rename Ï ğŸ™ = ğŸ™
rename Ï âŠ¥ = âŠ¥
rename Ï âŠ¤ = âŠ¤
rename Ï (ref (var x)) = ref (var (Ï x))
rename Ï (ref (ort x)) = ref (ort (Ï x))
rename Ï (Â¡ A) = Â¡ (rename Ï A)
rename Ï (Â¿ A) = Â¿ (rename Ï A)
rename Ï (A & B) = rename Ï A & rename Ï B
rename Ï (A âŠ• B) = rename Ï A âŠ• rename Ï B
rename Ï (A âŠ— B) = rename Ï A âŠ— rename Ï B
rename Ï (A â…‹ B) = rename Ï A â…‹ rename Ï B
rename Ï ($âˆ€ A) = $âˆ€ (rename (ext Ï) A)
rename Ï ($âˆƒ A) = $âˆƒ (rename (ext Ï) A)

exts : âˆ€{m n} -> (Fin m -> Type n) -> Fin (suc m) -> Type (suc n)
exts Ïƒ zero = ref (var zero)
exts Ïƒ (suc k) = rename suc (Ïƒ k)

data SubstN {m n} : (Ïƒ : Fin m -> Type n) -> Name m -> Type n -> Set where
  s-var : âˆ€{Ïƒ x A} -> Dual (Ïƒ x) A -> SubstN Ïƒ (var x) (Ïƒ x)
  s-ort : âˆ€{Ïƒ x A} -> Dual (Ïƒ x) A -> SubstN Ïƒ (ort x) A

data Subst {m n} : (Ïƒ : Fin m -> Type n) -> Type m -> Type n -> Set where
  s-ğŸ˜ : âˆ€{Ïƒ} -> Subst Ïƒ ğŸ˜ ğŸ˜
  s-ğŸ™ : âˆ€{Ïƒ} -> Subst Ïƒ ğŸ™ ğŸ™
  s-âŠ¥ : âˆ€{Ïƒ} -> Subst Ïƒ âŠ¥ âŠ¥
  s-âŠ¤ : âˆ€{Ïƒ} -> Subst Ïƒ âŠ¤ âŠ¤
  s-r : âˆ€{Ïƒ A x} -> SubstN Ïƒ x A -> Subst Ïƒ (ref x) A
  s-! : âˆ€{Ïƒ A A'} -> Subst Ïƒ A A' -> Subst Ïƒ (Â¡ A) (Â¡ A')
  s-? : âˆ€{Ïƒ A A'} -> Subst Ïƒ A A' -> Subst Ïƒ (Â¿ A) (Â¿ A')
  s-& : âˆ€{Ïƒ A A' B B'} -> Subst Ïƒ A A' -> Subst Ïƒ B B' -> Subst Ïƒ (A & B) (A' & B')
  s-âŠ• : âˆ€{Ïƒ A A' B B'} -> Subst Ïƒ A A' -> Subst Ïƒ B B' -> Subst Ïƒ (A âŠ• B) (A' âŠ• B')
  s-âŠ— : âˆ€{Ïƒ A A' B B'} -> Subst Ïƒ A A' -> Subst Ïƒ B B' -> Subst Ïƒ (A âŠ— B) (A' âŠ— B')
  s-â…‹ : âˆ€{Ïƒ A A' B B'} -> Subst Ïƒ A A' -> Subst Ïƒ B B' -> Subst Ïƒ (A â…‹ B) (A' â…‹ B')
  s-âˆƒ : âˆ€{Ïƒ A A'} -> Subst (exts Ïƒ) A A' -> Subst Ïƒ ($âˆƒ A) ($âˆƒ A')
  s-âˆ€ : âˆ€{Ïƒ A A'} -> Subst (exts Ïƒ) A A' -> Subst Ïƒ ($âˆ€ A) ($âˆ€ A')

make-subst : âˆ€{n} -> Type n -> Fin (suc n) -> Type n
make-subst A zero = A
make-subst A (suc k) = ref (var k)
